src/LifetimeMemoryPerms.v
@@ -13,6 +13,7 @@ From ITree Require Import
      ITree
      Eq.Eqit.
 
+
 From Heapster Require Import
      Utils
      Permissions
@@ -22,13 +23,17 @@ From Heapster Require Import
      MemoryPerms
      LifetimePerms
      Typing
-     SepStep.
+     SepStep
+     PermTypeProofs.
 
 From Paco Require Import
      paco.
 
+Import ITreeNotations.
 Import ListNotations.
+
 Open Scope list_scope.
+Open Scope itree_scope.
 (* end hide *)
 
 Section Perms.
@@ -151,15 +156,55 @@ Section Perms.
     apply pre_inv_bottom.
   Qed.
 
+  Definition when_ptr_Perms {A} (l : nat) (rw : RW) (p : Value) (a : A) (T : VPermType A)
+    : @Perms (Si * Ss) :=
+    match p with
+    | VNum _ => top_Perms
+    | VPtr p =>
+        meet_Perms (fun P => exists (v : Value),
+                        P = singleton_Perms
+                              (match rw with
+                               | R => when l (read_perm p v) (nonLifetime_read_perm _ _)
+                               | W => when l (write_perm p v) (nonLifetime_write_perm _ _)
+                               end) *
+                              (v :: T ▷ a))
+    end.
+
+  Definition when_ptr {A} (l : nat) '(rw, o, T) : VPermType A :=
+    {|
+      ptApp := fun x a => when_ptr_Perms l rw (offset x o) a T;
+    |}.
+
+  Definition finished_ptr_Perms {A} (l : nat) (rw : RW) (p : Value) (a : A) (T : VPermType A) : @Perms (Si * Ss) :=
+    match p with
+    | VNum _ => top_Perms
+    | VPtr p =>
+        meet_Perms (fun P => exists (v : Value),
+                        P = singleton_Perms
+                              (match rw with
+                               | R => lfinished l (read_perm p v) (nonLifetime_read_perm _ _)
+                               | W => lfinished l (write_perm p v) (nonLifetime_write_perm _ _)
+                               end) *
+                              (v :: T ▷ a))
+    end.
+
+  Definition finished_ptr {A} (l : nat) '(rw, o, T) : VPermType A :=
+    {|
+      ptApp := fun x a => finished_ptr_Perms l rw (offset x o) a T;
+    |}.
+
+  (*
   Lemma split_Perms_trueP b o l (P Q : @Perms (Si * Ss)) :
     (VPtr (b, o)) :: ptr(W, 0, trueP) ▷ tt * lowned_Perms l P Q ⊨
-      when_Perms l ((VPtr (b, o)) :: ptr(W, 0, trueP) ▷ tt) *
+      (VPtr (b, o)) :: when_ptr l (W, 0, trueP) ▷ tt *
       lowned_Perms l
-        (when_Perms l ((VPtr (b, o)) :: ptr(R, 0, trueP) ▷ tt) * P)
+        ((VPtr (b, o)) :: when_ptr l (R, 0, trueP) ▷ tt * P)
         (((VPtr (b, o)) :: ptr(W, 0, trueP) ▷ tt) * Q).
   Proof.
     intros p0 (p' & powned & Hp' & (r1 & r2 & Hr1 & Hr2 & Hr2' & Hsep' & Hr2'' & Hlte' & Hf) & Hsep & Hlte).
     destruct (nonLifetime_ptr _ _ _ _ trueP nonLifetime_trueP _ Hp') as (p & Hp & Hpp' & Hnlp & Hguarp & Hprep).
+    destruct Hp as (? & (v & ?) & Hx); subst.
+    rewrite sep_conj_Perms_commut in Hx. rewrite sep_conj_Perms_bottom_identity in Hx.
     exists (when l p Hnlp).
     assert (Hpr2 : p ⊥ r2).
     {
@@ -170,10 +215,15 @@ Section Perms.
       }
       symmetry. eapply separate_antimonotone; eauto. symmetry. auto.
     }
-    cbn in Hp.
     eexists (r1 ** owned l (p ** r2) (nonLifetime_sep_conj_perm _ _ Hnlp Hr2 Hpr2)).
     split; [| split; [| split]]; auto.
-    - apply when_perm_Perms; auto.
+    - eexists. split. eexists. reflexivity.
+      cbn in Hp'.
+      cbn. do 2 eexists. split; [| split; [| split]].
+      reflexivity. auto.
+      apply separate_bottom.
+      rewrite sep_conj_perm_bottom.
+      apply when_monotone. apply Hx.
     - exists r1, (p ** r2), Hr1, (nonLifetime_sep_conj_perm _ _ Hnlp Hr2 Hpr2), (guar_inv_sep_conj_perm _ _ Hguarp Hr2').
       split; [| split; [| split]].
       3: reflexivity.
@@ -184,9 +234,12 @@ Section Perms.
       }
       {
         apply sep_conj_Perms_perm; auto.
+        cbn. eexists. split. eexists. reflexivity.
+        rewrite sep_conj_Perms_commut. rewrite sep_conj_Perms_bottom_identity. apply Hx.
       }
       (** Precondition part *)
-      intros p1 (pw & q & (? & (pr & Hpr' & Hpr & ?) & Hlte''') & Hq' & Hsep''' & Hlte'') Hsep''; subst.
+      intros p1 (pw & q & (? & (v' & ?) & Hlte''') & Hq' & Hsep'' & Hlte'') Hsep'''; subst.
+      (* intros p1 (pw & q & (? & (pr & Hpr' & Hpr & ?) & Hlte''') & Hq' & Hsep''' & Hlte'') Hsep''; subst. *)
       cbn in Hlte'''.
       specialize (Hf _ Hq'). destruct Hf as (r & Hr & Hsep_step & Hpre).
       {
@@ -253,7 +306,154 @@ Section Perms.
       etransitivity. apply convert.
       apply sep_conj_perm_monotone; [| reflexivity]; auto.
   Qed.
+   *)
 
+  Lemma split_Perms_T {A} b o o' l (P Q : @Perms (Si * Ss)) (T : VPermType A) xs
+    (HT : forall xi xs, nonLifetime_Perms (xi :: T ▷ xs)) :
+    (VPtr (b, o)) :: ptr(W, o', T) ▷ xs * lowned_Perms l P Q ⊨
+      (VPtr (b, o) :: when_ptr l (W, o', T) ▷ xs) *
+      lowned_Perms l
+        ((VPtr (b, o) :: when_ptr l (R, o', trueP) ▷ tt) * P)
+        ((VPtr (b, o) :: ptr(W, o', trueP) ▷ tt) * Q).
+  Proof.
+    intros p0 (p' & powned & Hp' & (r1 & r2 & Hr1 & Hr2 & Hr2' & Hsep' & Hr2'' & Hlte' & Hf) & Hsep & Hlte).
+    destruct Hp' as (? & (v & ?) & Hv). subst.
+    destruct Hv as (pw & pt & Hpw & Hpt & Hsep'' & Hlte'').
+    destruct (HT _ _ _ Hpt) as (pt' & Hpt' & Hltept & Hnlpt & Hguarpt & Hprept).
+    assert (Hsepwrite : write_perm (b, o + o') v ⊥ r2).
+    {
+      eapply owned_sep; auto. apply nonLifetime_write_perm. apply guar_inv_write_perm.
+      eapply separate_antimonotone.
+      2: { etransitivity. apply lte_r_sep_conj_perm. eauto. }
+      symmetry.
+      eapply separate_antimonotone. 2: apply Hpw.
+      eapply separate_antimonotone.
+      2: { etransitivity. apply lte_l_sep_conj_perm. eauto. }
+      symmetry. auto.
+    }
+    exists (when l (write_perm (b, o + o') v) (nonLifetime_write_perm _ _) ** pt').
+    exists (r1 ** owned l (write_perm (b, o + o') v ** r2) (nonLifetime_sep_conj_perm _ _ (nonLifetime_write_perm _ _) Hr2 Hsepwrite)).
+    split; [| split; [| split]].
+    - cbn. eexists. split. eexists. reflexivity.
+      cbn. do 2 eexists. split. reflexivity.
+      split; [| split]; try reflexivity; auto.
+      apply sep_when; auto.
+      eapply separate_antimonotone. 2: apply Hltept.
+      symmetry. eapply separate_antimonotone; eauto.
+      symmetry; auto.
+    - exists r1, (write_perm (b, o + o') v ** r2), Hr1.
+      exists (nonLifetime_sep_conj_perm _ _ (nonLifetime_write_perm _ _) Hr2 Hsepwrite).
+      exists (guar_inv_sep_conj_perm _ _ (guar_inv_write_perm _ _) Hr2').
+      split; [| split; [| split]].
+      + apply sep_owned; auto. eapply separate_antimonotone. 2: apply Hpw.
+        eapply separate_antimonotone.
+        2: { etransitivity. apply lte_l_sep_conj_perm. apply Hlte''. }
+        symmetry. eapply separate_antimonotone; eauto.
+        etransitivity; eauto. apply lte_l_sep_conj_perm.
+      + apply sep_conj_Perms_perm; auto.
+        cbn. eexists. split. eexists. reflexivity.
+        rewrite sep_conj_Perms_commut.
+        rewrite sep_conj_Perms_bottom_identity.
+        cbn. reflexivity.
+      + reflexivity.
+      + intros p1 (pwhen & q & (? & (v' & ?) & Hlte''') & Hq' & Hsep''' & Hlte'''') Hsep''''; subst.
+        rewrite sep_conj_Perms_commut in Hlte'''.
+        rewrite sep_conj_Perms_bottom_identity in Hlte'''. cbn in Hlte'''.
+
+        specialize (Hf _ Hq'). destruct Hf as (r & Hr & Hsep_step & Hpre).
+        {
+          symmetry in Hsep''''.
+          eapply separate_antimonotone in Hsep''''; eauto.
+          eapply separate_antimonotone in Hsep''''; eauto.
+          2: apply lte_r_sep_conj_perm.
+          symmetry in Hsep''''.
+          eapply separate_antimonotone in Hsep''''; eauto.
+          apply sep_conj_perm_monotone. reflexivity.
+          apply owned_monotone. apply lte_r_sep_conj_perm.
+        }
+        exists ((write_perm (b, o + o') v') ** r). split; [| split].
+        * apply sep_conj_Perms_perm; auto.
+          -- cbn. eexists. split. eexists. reflexivity.
+             rewrite sep_conj_Perms_commut. rewrite sep_conj_Perms_bottom_identity.
+             cbn. reflexivity.
+          -- symmetry. apply Hsep_step.
+             eapply separate_write_perm.
+             symmetry. eauto.
+        * etransitivity.
+          -- apply sep_step_sep_conj_r; eauto. symmetry. auto.
+          -- apply sep_step_sep_conj_l; eauto. symmetry. apply Hsep_step. symmetry. auto.
+             eapply sep_step_write_perm.
+             apply sep_step_lte'; eauto. reflexivity.
+        * (** Precondition section *)
+          intros. split; [| split].
+          -- apply Hlte'''' in H. destruct H as (? & ? & ?).
+             apply Hlte''' in H. cbn in H.
+             rewrite lGetPut in H. setoid_rewrite nth_error_replace_list_index_eq in H.
+             setoid_rewrite HGetPut1 in H.
+             cbn. rewrite HGetPut1. symmetry. apply H; auto.
+          -- apply Hpre; auto. apply Hlte''''; auto.
+          -- symmetry. apply Hsep_step.
+             eapply separate_write_perm.
+             symmetry. eauto.
+    - (** everything is pairwise separate *)
+      apply separate_sep_conj_perm_4.
+      + apply sep_when; auto.
+        eapply separate_antimonotone. 2: apply Hltept.
+        symmetry.
+        eapply separate_antimonotone. 2: apply Hpw. symmetry. auto.
+      + apply sep_when; auto.
+        eapply separate_antimonotone.
+        2: { etransitivity. apply lte_l_sep_conj_perm. eauto. }
+        symmetry.
+        eapply separate_antimonotone. 2: apply Hpw.
+        eapply separate_antimonotone.
+        2: { etransitivity. apply lte_l_sep_conj_perm. eauto. }
+        symmetry. auto.
+      + apply when_owned_sep.
+      + eapply separate_antimonotone.
+        2: { etransitivity. apply lte_l_sep_conj_perm. eauto. }
+        symmetry.
+        eapply separate_antimonotone. 2: apply Hltept.
+        eapply separate_antimonotone.
+        2: { etransitivity. apply lte_r_sep_conj_perm. eauto. }
+        symmetry. auto.
+      + apply sep_owned; auto.
+        * eapply separate_antimonotone. 2: apply Hpw.
+          symmetry. eapply separate_antimonotone; eauto.
+        * eapply separate_antimonotone.
+          2: { etransitivity. apply lte_r_sep_conj_perm. eauto. }
+          symmetry. eapply separate_antimonotone. 2: apply Hltept.
+          eapply separate_antimonotone.
+          2: { etransitivity. apply lte_r_sep_conj_perm. eauto. }
+          symmetry. auto.
+      + apply sep_owned; auto.
+        eapply separate_antimonotone. 2: apply Hpw.
+        eapply separate_antimonotone.
+        2: { etransitivity. apply lte_l_sep_conj_perm. eauto. }
+        symmetry. eapply separate_antimonotone.
+        2: { etransitivity. apply lte_l_sep_conj_perm. eauto. }
+        auto.
+    - (** Shuffling around permissions using <= *)
+      etransitivity; eauto.
+      etransitivity. 2: apply sep_conj_perm_monotone; [reflexivity |].
+      2: apply Hlte'.
+      do 2 rewrite <- sep_conj_perm_assoc.
+      do 2 rewrite (sep_conj_perm_commut _ r1).
+      do 3 rewrite sep_conj_perm_assoc.
+      apply sep_conj_perm_monotone; [reflexivity |].
+
+      etransitivity. 2: apply sep_conj_perm_monotone; [| reflexivity]; eauto.
+      rewrite <- sep_conj_perm_assoc.
+      rewrite (sep_conj_perm_commut _ pt).
+      rewrite (sep_conj_perm_commut _ pt').
+      do 2 rewrite sep_conj_perm_assoc.
+      apply sep_conj_perm_monotone; [assumption |].
+
+      etransitivity. apply convert.
+      apply sep_conj_perm_monotone; [| reflexivity]; auto.
+  Qed.
+
+  (*
   Lemma split_Perms_eq b o y l (P Q : @Perms (Si * Ss)) :
     (VPtr (b, o)) :: ptr(W, 0, eqp y) ▷ tt * lowned_Perms l P Q ⊨
       when_Perms l ((VPtr (b, o)) :: ptr(W, 0, eqp y) ▷ tt) *
@@ -360,50 +560,14 @@ Section Perms.
       etransitivity. apply convert.
       apply sep_conj_perm_monotone; [| reflexivity]; auto.
   Qed.
+   *)
 
-  Definition when_ptr_Perms {A} (l : nat) (rw : RW) (p : Value) (a : A) (T : VPermType A)
-    : @Perms (Si * Ss) :=
-    match p with
-    | VNum _ => top_Perms
-    | VPtr p =>
-        meet_Perms (fun P => exists (v : Value),
-                        P = singleton_Perms
-                              (match rw with
-                               | R => when l (read_perm p v) (nonLifetime_read_perm _ _)
-                               | W => when l (write_perm p v) (nonLifetime_write_perm _ _)
-                               end) *
-                              (v :: T ▷ a))
-    end.
-
-  Definition when_ptr {A} (l : nat) '(rw, o, T) : VPermType A :=
-    {|
-      ptApp := fun x a => when_ptr_Perms l rw (offset x o) a T;
-    |}.
-
-  Definition finished_ptr_Perms {A} (l : nat) (rw : RW) (p : Value) (a : A) (T : VPermType A) : @Perms (Si * Ss) :=
-    match p with
-    | VNum _ => top_Perms
-    | VPtr p =>
-        meet_Perms (fun P => exists (v : Value),
-                        P = singleton_Perms
-                              (match rw with
-                               | R => lfinished l (read_perm p v) (nonLifetime_read_perm _ _)
-                               | W => lfinished l (write_perm p v) (nonLifetime_write_perm _ _)
-                               end) *
-                              (v :: T ▷ a))
-    end.
-
-  Definition finished_ptr {A} (l : nat) '(rw, o, T) : VPermType A :=
-    {|
-      ptApp := fun x a => finished_ptr_Perms l rw (offset x o) a T;
-    |}.
-
-  Lemma typing_end' {A} l b o (T : VPermType A) xs (HT : forall v a, nonLifetime_Perms (v :: T ▷ a)) :
+  Lemma typing_end_ptr {A} l b o (T : VPermType A) xs (HT : forall v a, nonLifetime_Perms (v :: T ▷ a)) :
     typing (specConfig := Ss)
       ((VPtr (b, o)) :: when_ptr l (W, 0, T) ▷ xs *
-         (lowned_Perms l (when_Perms l ((VPtr (b, o)) :: ptr(R, 0, trueP) ▷ tt))
+         (lowned_Perms l ((VPtr (b, o)) :: when_ptr l (R, 0, trueP) ▷ tt)
             ((VPtr (b, o)) :: ptr(W, 0, trueP) ▷ tt)))
-      (fun _ _ => (VPtr (b, o)) :: finished_ptr l (W, 0, T) ▷ xs)
+      (fun l' _ => (VPtr (b, o)) :: finished_ptr l' (W, 0, T) ▷ xs)
       (endLifetime l)
       (Ret tt).
   Proof.
@@ -424,11 +588,12 @@ Section Perms.
     specialize (Hf (when l (write_perm (b, o + 0) v) (nonLifetime_write_perm (b, o + 0) v))).
     destruct Hf as (q & Hq & Hsep_step & Hpre).
     {
-      apply when_perm_Perms. eexists. split. eexists. reflexivity. cbn.
+      eexists. split. eexists. reflexivity. cbn.
       do 2 eexists. split; [| split; [| split]]. 2: auto.
-      - apply read_lte_write.
+      - reflexivity.
       - apply separate_bottom.
-      - rewrite sep_conj_perm_bottom. reflexivity.
+      - rewrite sep_conj_perm_bottom. apply when_monotone.
+        apply read_lte_write.
     }
     {
       apply Hlte in Hpre''. destruct Hpre'' as (? & ? & ?).
@@ -518,111 +683,132 @@ Section Perms.
     eapply nonLifetime_sep_step. 2: eauto. auto.
   Qed.
 
-
-  Lemma split_Perms' b o l (P Q : @Perms (Si * Ss)) T (xs : Ss)
-    (HT : forall xi xs, nonLifetime_Perms (xi :: T ▷ xs)) :
-    (VPtr (b, o)) :: ptr(W, 0, T) ▷ xs * lowned_Perms l P Q ⊨
-      (VPtr (b, o)) :: when_ptr l (W, 0, T) ▷ xs *
-      lowned_Perms l
-        ((VPtr (b, o)) :: when_ptr l (R, 0, trueP) ▷ xs * P)
-        ((VPtr (b, o)) :: when_ptr l (W, 0, trueP) ▷ xs * Q).
+  Lemma partial_ptr b o l o' y P Q :
+    (VPtr (b, o) :: when_ptr l (W, o', eqp y) ▷ tt) *
+          lowned_Perms l
+            ((VPtr (b, o) :: when_ptr l (R, o', trueP) ▷ tt) * P)
+            ((VPtr (b, o) :: ptr(W, o', trueP) ▷ tt) * Q)
+            ⊨
+    lowned_Perms l P ((VPtr (b, o) :: ptr(W, o', eqp y) ▷ tt) * Q).
   Proof.
-    intros p0 (p' & powned & Hp' & (r1 & r2 & Hr1 & Hr2 & Hr2' & Hsep' & Hr2'' & Hlte' & Hf) & Hsep & Hlte).
-    destruct (nonLifetime_ptr _ _ _ _ T HT _ Hp') as (p'' & Hp'' & Hpp' & Hnlp & Hguarp).
-    destruct Hp'' as (? & (v & ?) & Hasdf). subst.
-    destruct Hasdf as (p & pt & Hp & Hpt & Hsep'' & Hlte'').
-    cbn in Hp.
-    exists (when l p'' Hnlp).
-    assert (Hpr2 : p ⊥ r2).
+    intros p0 (pw' & powned & (? & (v & ?) & Hpw') & (r1 & r2 & Hr1 & Hr2 & Hr2' & Hsep' & Hr2'' & Hlte' & Hf) & Hsep & Hlte). subst.
+    cbn in Hpw'.
+    destruct Hpw' as (pw & p' & Hpw & ? & Hsep'' & Hlte''). subst.
+    (* destruct (HP _ Hp') as (p & Hp & Hpp' & Hnlp & Hguarp). *)
+    exists (when l (write_perm (b, o + o') v) (nonLifetime_write_perm (b, o + o') v) ** r1), r2. eexists.
     {
-      eapply owned_sep; auto.
-      eapply separate_antimonotone.
-      2: {
-        etransitivity. apply lte_r_sep_conj_perm. eauto.
-      }
-      symmetry. eapply separate_antimonotone; eauto. symmetry. auto.
-    }
-    eexists (r1 ** owned l (p ** r2) (nonLifetime_sep_conj_perm _ _ Hnlp Hr2 Hpr2)).
-    split; [| split; [| split]]; auto.
-    - apply when_perm_Perms; auto.
-    - exists r1, (p ** r2), Hr1, (nonLifetime_sep_conj_perm _ _ Hnlp Hr2 Hpr2), (guar_inv_sep_conj_perm _ _ Hguarp Hr2').
-      split; [| split; [| split]].
-      3: reflexivity.
-      {
-        apply sep_owned; auto. eapply separate_antimonotone. 2: apply Hpp'.
-        symmetry. eapply separate_antimonotone. apply Hsep.
-        etransitivity; eauto. apply lte_l_sep_conj_perm.
-      }
-      {
-        apply sep_conj_Perms_perm; auto.
-      }
-      (** Precondition part *)
-      intros p1 (pw & q & (? & (pr & Hpr' & Hpr & ?) & Hlte''') & Hq' & Hsep''' & Hlte'') Hsep''; subst.
-      cbn in Hlte'''.
-      specialize (Hf _ Hq'). destruct Hf as (r & Hr & Hsep_step & Hpre).
-      {
-        symmetry in Hsep''.
-        eapply separate_antimonotone in Hsep''; eauto.
-        eapply separate_antimonotone in Hsep''; eauto.
-        2: apply lte_r_sep_conj_perm.
-        symmetry in Hsep''.
-        eapply separate_antimonotone in Hsep''; eauto.
-        apply sep_conj_perm_monotone. reflexivity.
-        apply owned_monotone. apply lte_r_sep_conj_perm.
-      }
-      cbn in Hp.
-      destruct Hp as (? & (v & ?) & Hx). subst. rewrite Nat.add_0_r in Hx.
-      rewrite sep_conj_Perms_commut in Hx. rewrite sep_conj_Perms_bottom_identity in Hx.
-      cbn in Hx.
 
-      destruct Hpr as (? & (v' & ?) & Hx'). subst. rewrite Nat.add_0_r in Hx'.
-      rewrite sep_conj_Perms_commut in Hx'. rewrite sep_conj_Perms_bottom_identity in Hx'.
-      cbn in Hx'.
-      exists ((write_perm (b, o) v') ** r). split; [| split].
-      + apply sep_conj_Perms_perm; auto.
-        * cbn. eexists. split. eexists. reflexivity.
-          rewrite Nat.add_0_r.
-          rewrite sep_conj_Perms_commut. rewrite sep_conj_Perms_bottom_identity.
-          cbn. reflexivity.
-        * symmetry. eapply separate_write_perm.
-          apply Hsep_step.
-          eapply separate_antimonotone.
-          2: apply Hx.
-          symmetry. auto.
-      + etransitivity.
-        * apply sep_step_sep_conj_r; eauto. symmetry. auto.
-        * apply sep_step_sep_conj_l; eauto. symmetry. apply Hsep_step. symmetry. auto.
-          eapply sep_step_write_perm.
-          apply sep_step_lte'; eauto.
-      + intros. split; [| split]; auto.
-        * apply Hlte'' in H. destruct H as (? & ? & ?).
-          apply Hlte''' in H. cbn in H.
-          rewrite lGetPut in H. setoid_rewrite nth_error_replace_list_index_eq in H.
-          apply Hx' in H. cbn in *.
-          rewrite HGetPut1 in H |- *; auto. right. reflexivity.
-        * apply Hpre; auto. apply Hlte''; auto.
-        * symmetry. apply Hsep_step.
-          eapply separate_write_perm.
-          eapply separate_antimonotone. symmetry. apply Hpr2. apply Hx.
-    - apply separate_sep_conj_perm.
-      + apply sep_when; auto.
-        symmetry.
-        eapply separate_antimonotone. 2: apply Hpp'.
-        symmetry.
-        eapply separate_antimonotone. apply Hsep. etransitivity; eauto.
-        apply lte_l_sep_conj_perm.
-      + apply when_owned_sep.
-      + symmetry. apply sep_owned; auto. eapply separate_antimonotone. 2: apply Hpp'.
-        symmetry. eapply separate_antimonotone. apply Hsep.
+    }
+    exists Hr2, Hr2'. split.
+    {
+      symmetry. apply separate_sep_conj_perm.
+      - eapply separate_antimonotone; eauto.
+        symmetry. eapply separate_antimonotone; eauto.
+        etransitivity; eauto. apply lte_r_sep_conj_perm.
+      - symmetry. auto.
+      - eapply separate_antimonotone. 2: apply Hpp'.
+        symmetry. eapply separate_antimonotone; eauto.
         etransitivity; eauto. apply lte_l_sep_conj_perm.
-    - etransitivity; eauto.
-      etransitivity. 2: apply sep_conj_perm_monotone; [reflexivity |].
-      2: apply Hlte'.
-      do 2 rewrite <- sep_conj_perm_assoc.
-      do 2 rewrite (sep_conj_perm_commut _ r1).
-      do 2 rewrite sep_conj_perm_assoc.
-      apply sep_conj_perm_monotone; [reflexivity |].
-      etransitivity. apply convert.
-      apply sep_conj_perm_monotone; [| reflexivity]; auto.
+    }
+    split; [| split]; auto.
+    {
+      etransitivity; eauto. rewrite sep_conj_perm_assoc.
+      apply sep_conj_perm_monotone; auto; reflexivity.
+    }
+    intros q Hq Hsep''.
+    rewrite sep_conj_perm_assoc in Hsep''.
+    specialize (Hf (p ** q)).
+    destruct Hf as (r & Hr & Hsep_step & Hpre).
+    - apply sep_conj_Perms_perm; auto. symmetry.
+      eapply separate_antimonotone; eauto.
+      apply lte_l_sep_conj_perm.
+    - symmetry. apply separate_sep_conj_perm.
+      + eapply separate_antimonotone; eauto.
+        symmetry. eapply separate_antimonotone; eauto.
+      + symmetry. eapply separate_antimonotone; eauto. apply lte_r_sep_conj_perm.
+      + eapply separate_antimonotone; eauto. apply lte_l_sep_conj_perm.
+    - exists r. split; [| split]; auto.
+      intros. apply Hpre.
+      + destruct H0. split; [| split]; auto.
+        symmetry. eapply separate_antimonotone; eauto. apply lte_l_sep_conj_perm.
+      + apply H0.
   Qed.
+
+  Lemma ex3_typing b o xs :
+    typing
+      (lifetime_Perms * (VPtr (b, o)) :: ptr (W, 0, IsNat Si Ss) ▷ xs)
+      (fun l _ => lifetime_Perms * (VPtr (b, o)) :: finished_ptr l (W, 0, IsNat Si Ss) ▷ xs)
+      (l <- beginLifetime ;; Ret tt ;; endLifetime l)
+      (Ret tt ;; Ret tt ;; Ret tt).
+  Proof.
+    eapply typing_bind.
+    { apply typing_frame. apply typing_begin. }
+    intros. unfold id.
+    rewrite sep_conj_Perms_commut.
+    rewrite sep_conj_Perms_assoc.
+    setoid_rewrite (sep_conj_Perms_commut lifetime_Perms).
+    apply typing_frame.
+
+    eapply typing_bind with (Q := (fun _ _ => (VPtr (b, o) :: when_ptr r1 (W, 0, IsNat Si Ss) ▷ xs *
+     lowned_Perms r1 (VPtr (b, o) :: when_ptr r1 (R, 0, trueP) ▷ tt * bottom_Perms)
+       (VPtr (b, o) :: ptr (W, 0, trueP) ▷ tt * bottom_Perms)))).
+    {
+      eapply typing_lte with (Q := fun _ _ => VPtr (b, o) :: when_ptr r1 (W, 0, IsNat Si Ss) ▷ xs *
+   lowned_Perms r1 (VPtr (b, o) :: when_ptr r1 (R, 0, trueP) ▷ tt * bottom_Perms)
+     (VPtr (b, o) :: ptr (W, 0, trueP) ▷ tt * bottom_Perms)).
+      2: {
+        apply split_Perms_T.
+        repeat intro.
+        cbn in *. subst. exists bottom_perm.
+        split; [| split; [| split; [| split]]]; auto.
+        apply bottom_perm_is_bottom.
+        apply nonLifetime_bottom.
+        apply guar_inv_bottom.
+        apply pre_inv_bottom.
+      }
+
+      apply typing_ret. reflexivity.
+      reflexivity.
+    }
+    intros _ _. apply typing_end_ptr.
+
+    eapply typing_bind with (Q:=(fun _ _ : unit =>
+                                   VPtr (b, o) :: ptr (W, 1, IsNat Si Ss) ▷ xs2 *
+                                     lowned_Perms r1 bottom_Perms bottom_Perms *
+                                     VPtr (b, o) :: ptr (W, 0, IsNat Si Ss) ▷ xs1)).
+    { rewrite <- sep_conj_Perms_assoc.
+      rewrite (sep_conj_Perms_commut _ (lowned_Perms _ _ _)).
+      rewrite sep_conj_Perms_commut.
+      apply typing_frame.
+      eapply typing_lte.
+      2: { rewrite sep_conj_Perms_commut. eapply split_Perms_T. admit. }
+      apply typing_ret.
+      reflexivity.
+    }
+    { rewrite
+      }
+
+    eapply typing_lte with (Q:=(fun _ _ : unit =>
+                                  VPtr (b, o) :: ptr (W, 0, IsNat Si Ss) ▷ xs1 *
+                                    VPtr (b, o) :: ptr (W, 1, IsNat Si Ss) ▷ xs2)).
+    3: reflexivity.
+    2: {
+      rewrite <- sep_conj_Perms_assoc.
+      etransitivity.
+      apply lte_r_sep_conj_Perms.
+      apply split_Perms_T.
+      admit.
+    }
+    eapply typing_lte with (Q:=(fun _ _ : unit =>
+                                  VPtr (b, o) :: ptr (W, 0, IsNat Si Ss) ▷ xs1 *
+                                    VPtr (b, o) :: ptr (W, 1, IsNat Si Ss) ▷ xs2)).
+    3: reflexivity.
+    2: {
+      apply split_Perms_T.
+      admit.
+    }
+
+
+  Qed.
+
 End Perms.
